Clean up demos a bit

coq/PerformanceDemos/do_n_binder.v
@@ -10,45 +10,12 @@
 
 (** See also COQBUG(https://github.com/coq/coq/issues/8244) *)
 
-(** TODO: Maybe we should organize files by the performance criterion
-     and not the tested tactic? *)
-Fixpoint letn n (x : nat) (k : nat -> Prop) :=
-  match n with
-  | O => k x
-  | S n =>
-    let x := S x in
-    letn n x k
-  end.
-
 Fixpoint foralln n (x : nat) (k : nat -> Prop) :=
   match n with
   | O => k x
   | S n =>
     forall x : nat, foralln n x k
   end.
-
-Goal letn 250 O (fun _ => True). cbv beta iota delta [letn]. Time intros. Time Optimize Proof. exact I. Qed.
-(*Finished transaction in 0.029 secs (0.022u,0.006s) (successful)
-Evars: 253 -> 1
-Finished transaction in 0.012 secs (0.012u,0.s) (successful) *)
-Goal letn 500 O (fun _ => True). cbv beta iota delta [letn]. Time intros. Time Optimize Proof. exact I. Qed.
-(* Finished transaction in 0.055 secs (0.054u,0.s) (successful)
-Evars: 503 -> 1
-Finished transaction in 0.123 secs (0.122u,0.s) (successful) *)
-Goal letn 1000 O (fun _ => True). cbv beta iota delta [letn]. Time intros. Time Optimize Proof. exact I. Qed.
-(* Finished transaction in 0.264 secs (0.257u,0.006s) (successful)
-Evars: 1003 -> 1
-Finished transaction in 0.73 secs (0.726u,0.003s) (successful) *)
-Goal letn 2000 O (fun _ => True). cbv beta iota delta [letn]. Time intros. Time Optimize Proof. exact I. Qed.
-(* Finished transaction in 1.09 secs (1.077u,0.009s) (successful)
-Evars: 2003 -> 1
-Finished transaction in 6.754 secs (6.741u,0.006s) (successful) *)
-(*
-Goal letn 4000 O (fun _ => True). cbv beta iota delta [letn]. Time intros. Time Optimize Proof. exact I. Qed.
-(* Finished transaction in 4.324 secs (4.235u,0.079s) (successful)
-Evars: 4003 -> 1
-Finished transaction in 68.641 secs (68.531u,0.073s) (successful) *)
- *)
 
 Goal foralln 250 O (fun _=> True). cbv beta iota delta [foralln]. Time intros. Time Optimize Proof. exact I. Qed.
 (* Finished transaction in 0.034 secs (0.034u,0.s) (successful)
