coq/PerformanceDemos/do_n_let_binder.v
@@ -1,0 +1,83 @@
+(** * Performance Criterion: Adding a new let binder underneath n lets should be Õ(1) *)
+
+(** We can establish this criterion in three ways: using the proof
+    engine to add a new let binder either (a) via [pose] or (b) via
+    [intro], or (c) looking at the marginal increase of adding another
+    let binder to a term and re-type-checking it. *)
+
+(** Note that in Coq, this is severely complicated by the overhead of
+    fresh name generation. *)
+
+(** See also COQBUG(https://github.com/coq/coq/issues/8244) *)
+
+Goal True.
+  Time (do 1000 pose I).
+  (* Finished transaction in 0.293 secs (0.289u,0.003s) (successful) *)
+  Time (do 1000 pose I).
+  (* Finished transaction in 0.746 secs (0.734u,0.011s) (successful) *)
+  Time (do 1000 pose I).
+  (* Finished transaction in 1.29 secs (1.27u,0.019s) (successful) *)
+Abort.
+
+Ltac make n :=
+  lazymatch n with
+  | O => uconstr:(I)
+  | S ?n => let rest := make n in
+            uconstr:(let _ := I in rest)
+  end.
+
+Ltac make_and_check n :=
+  restart_timer;
+  let res := make n in
+  finish_timing ("Tactic call make");
+  restart_timer;
+  let res := constr:(res) in
+  finish_timing ("Tactic call constr");
+  idtac.
+
+Goal True.
+  make_and_check 1000.
+  (* Tactic call make ran for 0.037 secs (0.022u,0.015s)
+Tactic call constr ran for 0.011 secs (0.011u,0.s)
+   *)
+  make_and_check 2000.
+  (* Tactic call make ran for 0.051 secs (0.045u,0.005s)
+Tactic call constr ran for 0.047 secs (0.047u,0.s)
+*)
+  make_and_check 4000.
+  (* Tactic call make ran for 0.094 secs (0.094u,0.s)
+Tactic call constr ran for 0.205 secs (0.205u,0.s)
+   *)
+Abort.
+
+
+Fixpoint letn n (x : nat) (k : nat -> Prop) :=
+  match n with
+  | O => k x
+  | S n =>
+    let x := S x in
+    letn n x k
+  end.
+
+Goal letn 250 O (fun _ => True). cbv beta iota delta [letn]. Time intros. Time Optimize Proof. exact I. Qed.
+(*Finished transaction in 0.029 secs (0.022u,0.006s) (successful)
+Evars: 253 -> 1
+Finished transaction in 0.012 secs (0.012u,0.s) (successful) *)
+Goal letn 500 O (fun _ => True). cbv beta iota delta [letn]. Time intros. Time Optimize Proof. exact I. Qed.
+(* Finished transaction in 0.055 secs (0.054u,0.s) (successful)
+Evars: 503 -> 1
+Finished transaction in 0.123 secs (0.122u,0.s) (successful) *)
+Goal letn 1000 O (fun _ => True). cbv beta iota delta [letn]. Time intros. Time Optimize Proof. exact I. Qed.
+(* Finished transaction in 0.264 secs (0.257u,0.006s) (successful)
+Evars: 1003 -> 1
+Finished transaction in 0.73 secs (0.726u,0.003s) (successful) *)
+Goal letn 2000 O (fun _ => True). cbv beta iota delta [letn]. Time intros. Time Optimize Proof. exact I. Qed.
+(* Finished transaction in 1.09 secs (1.077u,0.009s) (successful)
+Evars: 2003 -> 1
+Finished transaction in 6.754 secs (6.741u,0.006s) (successful) *)
+(*
+Goal letn 4000 O (fun _ => True). cbv beta iota delta [letn]. Time intros. Time Optimize Proof. exact I. Qed.
+(* Finished transaction in 4.324 secs (4.235u,0.079s) (successful)
+Evars: 4003 -> 1
+Finished transaction in 68.641 secs (68.531u,0.073s) (successful) *)
+ *)
